refactor: EqSb part 1

GroupoidModel/Russell_PER_MS/Substitution.lean
@@ -116,29 +116,37 @@ theorem EqTm.le_univMax {Γ t u A l} : Γ ⊢[l] t ≡ u : A → l ≤ univMax :
 
 /-! ## Admissibility of renaming -/
 
-/-- The renaming `ξ : Δ ⟶ Γ` is well-formed. -/
+/-- The renaming `ξ : Δ ⟶ Γ` is well-formed.
+
+This notion is only useful as an intermediate step
+in establishing admissibility of substitution.
+After that, always use `WfSb`. -/
+@[irreducible]
 def WfRen (Δ : Ctx) (ξ : Nat → Nat) (Γ : Ctx) :=
   ∀ {i A l}, Lookup Γ i A l → Lookup Δ (ξ i) (A.rename ξ) l
 
 namespace WfRen
 
-theorem id (Γ) : WfRen Γ id Γ :=
-  fun lk => by convert lk; autosubst
+theorem lookup {Δ Γ A ξ i l} : WfRen Δ ξ Γ → Lookup Γ i A l → Lookup Δ (ξ i) (A.rename ξ) l := by
+  unfold WfRen; intro h; exact h
+
+theorem id (Γ) : WfRen Γ id Γ := by
+  unfold WfRen; intro _ _ _ lk; convert lk; autosubst
 
 theorem wk (Γ A l) : WfRen ((A,l) :: Γ) Nat.succ Γ := by
-  intro _ _ _ lk
+  unfold WfRen; intro _ _ _ lk
   convert Lookup.succ _ _ lk
   autosubst
 
 theorem comp {Θ Δ Γ ξ₁ ξ₂} : WfRen Θ ξ₁ Δ → WfRen Δ ξ₂ Γ → WfRen Θ (fun i => ξ₁ (ξ₂ i)) Γ := by
-  intro wf₁ wf₂ _ _ _ lk
+  unfold WfRen; intro wf₁ wf₂ _ _ _ lk
   convert wf₁ <| wf₂ lk using 1
   autosubst
   congr 1
 
 theorem upr {Δ Γ A ξ l} : WfRen Δ ξ Γ →
     WfRen ((A.rename ξ, l) :: Δ) (Expr.upr ξ) ((A, l) :: Γ) := by
-  intro wf _ _ _ lk
+  unfold WfRen; intro wf _ _ _ lk
   cases lk
   . rw [show (A.subst Expr.wk).rename (Expr.upr ξ) = (A.rename ξ).subst Expr.wk by autosubst]
     apply Lookup.zero
@@ -165,7 +173,7 @@ theorem rename_all :
   mutual_induction
   case snoc => exact True.intro
   all_goals try dsimp [Expr.rename] at *
-  case bvar sb => apply WfTm.bvar _ (sb _) <;> assumption
+  case bvar ξ => apply WfTm.bvar _ (ξ.lookup _) <;> assumption
   grind_cases
   -- Cases that didn't go through automatically.
   case snd' => rw [ih_subst]; apply WfTm.snd' <;> grind
@@ -193,62 +201,85 @@ theorem WfCtx.lookup_wf {Γ i A l} : WfCtx Γ → Lookup Γ i A l → Γ ⊢[l] 
 
 /-! ## Admissibility of substitution -/
 
-/-- The substitution `σ : Δ ⟶ Γ` is well-formed
-and preserves bound variables' types.
+/-- The substitution `σ : Δ ⟶ Γ` is well-formed.
 
 This is a functional definition as in the Autosubst paper,
-but with preservation data added for the inductive argument.
+but with more preservation data added so that we can use this
+before proving admissibility of substitution and inversion.
+The additional data is an implementation detail;
+`WfSb` should not be unfolded outside of this module.
 
 A common alternative is to use an inductive characterization. -/
 @[irreducible]
 def WfSb (Δ : Ctx) (σ : Nat → Expr) (Γ : Ctx) :=
-  ∀ {i A l}, Lookup Γ i A l → (Δ ⊢[l] A.subst σ) ∧ (Δ ⊢[l] σ i : A.subst σ)
+  WfCtx Δ ∧ WfCtx Γ ∧ ∀ {i A l}, Lookup Γ i A l → (Δ ⊢[l] A.subst σ) ∧ (Δ ⊢[l] σ i : A.subst σ)
 
 namespace WfSb
 
-theorem lookup {Δ Γ A σ i l} : WfSb Δ σ Γ → Lookup Γ i A l → Δ ⊢[l] σ i : A.subst σ :=
-  fun h lk => by unfold WfSb at h; exact h lk |>.2
+theorem wf_dom {Δ Γ σ} : WfSb Δ σ Γ → WfCtx Δ := by
+  unfold WfSb; intro h; exact h.1
 
-theorem ofRen {Δ Γ ξ} : WfCtx Δ → WfRen Δ ξ Γ → WfSb Δ (Expr.ofRen ξ) Γ := by
+theorem wf_cod {Δ Γ σ} : WfSb Δ σ Γ → WfCtx Γ := by
+  unfold WfSb; intro h; exact h.2.1
+
+theorem lookup {Δ Γ A σ i l} : WfSb Δ σ Γ → Lookup Γ i A l → Δ ⊢[l] σ i : A.subst σ :=
+  fun h lk => by unfold WfSb at h; exact h.2.2 lk |>.2
+
+theorem ofRen {Δ Γ ξ} : WfCtx Δ → WfCtx Γ → WfRen Δ ξ Γ → WfSb Δ (Expr.ofRen ξ) Γ := by
   unfold WfSb
-  intro h h' _ _ _ lk
+  intro Δ Γ ξ
+  refine ⟨Δ, Γ, fun lk => ?_⟩
   constructor
   . rw [← Expr.rename_eq_subst_ofRen]
-    exact h.lookup_wf (h' lk)
-  . convert WfTm.bvar h (h' lk) using 1
+    exact Δ.lookup_wf (ξ.lookup lk)
+  . convert WfTm.bvar Δ (ξ.lookup lk) using 1
     autosubst
 
 theorem id {Γ} : WfCtx Γ → WfSb Γ Expr.bvar Γ :=
-  fun h => ofRen h (WfRen.id Γ)
+  fun h => ofRen h h (WfRen.id Γ)
 
 end WfSb
 
-/-- The substitutions `σ σ' : Δ ⟶ Γ` are definitionally equal,
-preserve variables' types, and are congruent on those types. -/
+/-- The substitutions `σ σ' : Δ ⟶ Γ` are definitionally equal. -/
 @[irreducible]
 def EqSb (Δ : Ctx) (σ σ' : Nat → Expr) (Γ : Ctx) :=
-  ∀ {i A l}, Lookup Γ i A l →
-    (Δ ⊢[l] A.subst σ) ∧ (Δ ⊢[l] A.subst σ') ∧ (Δ ⊢[l] A.subst σ ≡ A.subst σ') ∧
-    (Δ ⊢[l] σ i ≡ σ' i : A.subst σ)
+  WfCtx Δ ∧ WfCtx Γ ∧
+    ∀ {i A l}, Lookup Γ i A l →
+      (Δ ⊢[l] A.subst σ) ∧ (Δ ⊢[l] A.subst σ') ∧ (Δ ⊢[l] A.subst σ ≡ A.subst σ') ∧
+      (Δ ⊢[l] σ i ≡ σ' i : A.subst σ)
 
 namespace EqSb
 
+theorem wf_dom {Δ Γ σ σ'} : EqSb Δ σ σ' Γ → WfCtx Δ := by
+  unfold EqSb; intro h; exact h.1
+
+theorem wf_cod {Δ Γ σ σ'} : EqSb Δ σ σ' Γ → WfCtx Γ := by
+  unfold EqSb; intro h; exact h.2.1
+
+theorem lookup {Δ Γ A σ σ' i l} : EqSb Δ σ σ' Γ → Lookup Γ i A l →
+    Δ ⊢[l] σ i ≡ σ' i : A.subst σ :=
+  fun h lk => by unfold EqSb at h; exact h.2.2 lk |>.2.2.2
+
 theorem refl {Δ Γ σ} : WfSb Δ σ Γ → EqSb Δ σ σ Γ := by
   unfold WfSb EqSb
-  intro h _ _ _ lk
-  exact ⟨(h lk).1, (h lk).1, EqTp.refl_tp (h lk).1, EqTm.refl_tm (h lk).2⟩
+  intro σ
+  refine ⟨σ.1, σ.2.1, fun lk => ?_⟩
+  exact ⟨(σ.2.2 lk).1, (σ.2.2 lk).1, EqTp.refl_tp (σ.2.2 lk).1, EqTm.refl_tm (σ.2.2 lk).2⟩
 
 theorem symm {Δ Γ σ σ'} : EqSb Δ σ σ' Γ → EqSb Δ σ' σ Γ := by
-  grind [EqSb, EqTp.symm_tp, EqTm.symm_tm', EqTm.conv_tm]
+  unfold EqSb; grind [EqTp.symm_tp, EqTm.symm_tm', EqTm.conv_tm]
 
 theorem trans {Δ Γ σ σ' σ''} : EqSb Δ σ σ' Γ → EqSb Δ σ' σ'' Γ → EqSb Δ σ σ'' Γ := by
   unfold EqSb
-  intro h h' _ _ _ lk
+  intro h h'
+  refine ⟨h.1, h.2.1, fun lk => ?_⟩
   exact ⟨
-    (h lk).1,
-    (h' lk).2.1,
-    (h lk).2.2.1.trans_tp (h' lk).2.2.1,
-    (h lk).2.2.2.trans_tm' (h lk).1 ((h' lk).2.2.2.conv_tm (h lk).2.2.1.symm_tp)
+    (h.2.2 lk).1,
+    (h'.2.2 lk).2.1,
+    (h.2.2 lk).2.2.1.trans_tp (h'.2.2 lk).2.2.1,
+    (h.2.2 lk).2.2.2.trans_tm'
+      (h.2.2 lk).1
+      ((h'.2.2 lk).2.2.2.conv_tm (h.2.2 lk).2.2.1.symm_tp)
   ⟩
 
 end EqSb
@@ -263,52 +294,55 @@ we define better versions with fewer arguments. -/
 namespace SubstProof
 
 theorem wfSb_wk {Γ A l} : WfCtx Γ → Γ ⊢[l] A → WfSb ((A,l) :: Γ) Expr.wk Γ :=
-  fun h h' => WfSb.ofRen (h.snoc h') (WfRen.wk _ _ _)
+  fun h h' => WfSb.ofRen (h.snoc h') h (WfRen.wk ..)
 
-theorem wfSb_snoc {Δ Γ A t σ l} : WfSb Δ σ Γ → Δ ⊢[l] A.subst σ → Δ ⊢[l] t : A.subst σ →
+theorem wfSb_snoc {Δ Γ A t σ l} : WfSb Δ σ Γ →
+    Γ ⊢[l] A → Δ ⊢[l] A.subst σ → Δ ⊢[l] t : A.subst σ →
     WfSb Δ (Expr.snoc σ t) ((A,l) :: Γ) := by
-  unfold WfSb
-  intro σ Aσ t _ _ _ lk
+  unfold WfSb; intro σ A Aσ t
+  refine ⟨σ.1, σ.2.1.snoc A, fun lk => ?_⟩
   cases lk
   . constructor
     . convert Aσ using 1; autosubst
-    . autosubst; grind [WfSb]
+    . autosubst; grind
   next lk =>
     constructor
-    . convert (σ lk).1 using 1; autosubst
-    . autosubst; grind [WfSb]
+    . convert (σ.2.2 lk).1 using 1; autosubst
+    . autosubst; grind
 
-theorem wfSb_up_of_eq {Δ Γ A Aσ σ l} : WfCtx Δ → WfSb Δ σ Γ →
-    Δ ⊢[l] Aσ → Δ ⊢[l] A.subst σ → Δ ⊢[l] Aσ ≡ A.subst σ →
+theorem wfSb_up_of_eq {Δ Γ A Aσ σ l} : WfSb Δ σ Γ →
+    Γ ⊢[l] A → Δ ⊢[l] Aσ → Δ ⊢[l] A.subst σ → Δ ⊢[l] Aσ ≡ A.subst σ →
     WfSb ((Aσ, l) :: Δ) (Expr.up σ) ((A,l) :: Γ) := by
-  unfold WfSb
-  intro Δwf ΔσΓ ΔAσ ΔAσ' ΔAσeq _ _ _ lk
-  have ΔAσwf := Δwf.snoc ΔAσ
+  unfold WfSb; intro σ A Aσ Aσ' Aσeq
+  have ΔAσ := σ.1.snoc Aσ
+  refine ⟨ΔAσ, σ.2.1.snoc A, fun lk => ?_⟩
   cases lk
   . constructor
-    . convert rename_all.2.1 ΔAσ' ΔAσwf (@WfRen.wk _ _ _) using 1 <;> autosubst
-    . apply WfTm.conv (A := Aσ.subst Expr.wk)
+    . convert rename_all.2.1 Aσ' ΔAσ (WfRen.wk ..) using 1 <;> autosubst
+    . apply WfTm.conv (A := Expr.subst Expr.wk _)
       . rw [Expr.up_eq_snoc]
-        apply WfTm.bvar ΔAσwf
+        apply WfTm.bvar ΔAσ
         apply Lookup.zero
-      . convert rename_all.2.2.1 ΔAσeq ΔAσwf (@WfRen.wk _ _ _) using 1 <;> autosubst
+      . convert rename_all.2.2.1 Aσeq ΔAσ (WfRen.wk ..) using 1 <;> autosubst
   next lk =>
     constructor
-    . convert rename_all.2.1 (ΔσΓ lk).1 ΔAσwf (@WfRen.wk _ _ _) using 1 <;> autosubst
+    . convert rename_all.2.1 (σ.2.2 lk).1 ΔAσ (WfRen.wk ..) using 1 <;> autosubst
     . rw [Expr.up_eq_snoc]
-      convert rename_all.2.2.2.1 (ΔσΓ lk).2 ΔAσwf (@WfRen.wk _ _ _) using 1 <;> autosubst
+      convert rename_all.2.2.2.1 (σ.2.2 lk).2 ΔAσ (WfRen.wk ..) using 1 <;> autosubst
       rw [Expr.comp]
 
-theorem wfSb_up {Δ Γ A σ l} : WfCtx Δ → WfSb Δ σ Γ → Δ ⊢[l] A.subst σ →
+theorem wfSb_up {Δ Γ A σ l} : WfSb Δ σ Γ →
+    Γ ⊢[l] A → Δ ⊢[l] A.subst σ →
     WfSb ((A.subst σ, l) :: Δ) (Expr.up σ) ((A,l) :: Γ) :=
-  fun Δwf ΔσΓ ΔAσ => wfSb_up_of_eq Δwf ΔσΓ ΔAσ ΔAσ (EqTp.refl_tp ΔAσ)
+  fun ΔσΓ ΓA ΔAσ => wfSb_up_of_eq ΔσΓ ΓA ΔAσ ΔAσ (EqTp.refl_tp ΔAσ)
 
 theorem eqSb_snoc {Δ Γ A t t' σ σ' l} : EqSb Δ σ σ' Γ →
-    Δ ⊢[l] A.subst σ → Δ ⊢[l] A.subst σ' → Δ ⊢[l] A.subst σ ≡ A.subst σ' →
+    Γ ⊢[l] A → Δ ⊢[l] A.subst σ → Δ ⊢[l] A.subst σ' → Δ ⊢[l] A.subst σ ≡ A.subst σ' →
     Δ ⊢[l] t ≡ t' : A.subst σ →
     EqSb Δ (Expr.snoc σ t) (Expr.snoc σ' t') ((A,l) :: Γ) := by
   unfold EqSb
-  intro σσ' Aσ Aσ' AσAσ' tt' _ _ _ lk
+  intro σσ' A Aσ Aσ' AσAσ' tt'
+  refine ⟨σσ'.1, σσ'.2.1.snoc A, fun lk => ?_⟩
   cases lk
   . repeat any_goals apply And.intro
     . convert Aσ using 1; autosubst
@@ -317,66 +351,67 @@ theorem eqSb_snoc {Δ Γ A t t' σ σ' l} : EqSb Δ σ σ' Γ →
     . convert tt' using 1; autosubst
   next lk =>
     repeat any_goals apply And.intro
-    . convert (σσ' lk).1 using 1; autosubst
-    . convert (σσ' lk).2.1 using 1; autosubst
-    . convert (σσ' lk).2.2.1 using 1 <;> autosubst
-    . convert (σσ' lk).2.2.2 using 1 <;> autosubst
+    . convert (σσ'.2.2 lk).1 using 1; autosubst
+    . convert (σσ'.2.2 lk).2.1 using 1; autosubst
+    . convert (σσ'.2.2 lk).2.2.1 using 1 <;> autosubst
+    . convert (σσ'.2.2 lk).2.2.2 using 1 <;> autosubst
 
-theorem eqSb_up {Δ Γ A σ σ' l} : WfCtx Δ → EqSb Δ σ σ' Γ →
-    Δ ⊢[l] A.subst σ → Δ ⊢[l] A.subst σ' → Δ ⊢[l] A.subst σ ≡ A.subst σ' →
+theorem eqSb_up {Δ Γ A σ σ' l} : EqSb Δ σ σ' Γ →
+    Γ ⊢[l] A → Δ ⊢[l] A.subst σ → Δ ⊢[l] A.subst σ' → Δ ⊢[l] A.subst σ ≡ A.subst σ' →
     EqSb ((A.subst σ, l) :: Δ) (Expr.up σ) (Expr.up σ') ((A,l) :: Γ) := by
   unfold EqSb
-  intro Δwf ΔσΓ ΔAσ ΔAσ' ΔAσeq _ _ _ lk
-  have ΔAσwf := Δwf.snoc ΔAσ
+  intro σσ' A Aσ Aσ' Aσeq
+  have ΔAσ := σσ'.1.snoc Aσ
+  refine ⟨ΔAσ, σσ'.2.1.snoc A, fun lk => ?_⟩
   cases lk
   . repeat any_goals apply And.intro
-    . convert rename_all.2.1 ΔAσ ΔAσwf (@WfRen.wk _ _ _) using 1 <;> autosubst
-    . convert rename_all.2.1 ΔAσ' ΔAσwf (@WfRen.wk _ _ _) using 1 <;> autosubst
-    . convert rename_all.2.2.1 ΔAσeq ΔAσwf (@WfRen.wk _ _ _) using 1 <;> autosubst
+    . convert rename_all.2.1 Aσ ΔAσ (WfRen.wk ..) using 1 <;> autosubst
+    . convert rename_all.2.1 Aσ' ΔAσ (WfRen.wk ..) using 1 <;> autosubst
+    . convert rename_all.2.2.1 Aσeq ΔAσ (WfRen.wk ..) using 1 <;> autosubst
     . rw [Expr.up_eq_snoc σ, Expr.up_eq_snoc σ']
       apply EqTm.refl_tm
-      apply WfTm.bvar ΔAσwf
+      apply WfTm.bvar ΔAσ
       convert Lookup.zero .. using 1
       autosubst
   next lk =>
-    have := ΔσΓ lk
+    have := σσ'.2.2 lk
     repeat any_goals apply And.intro
-    . convert rename_all.2.1 this.1 ΔAσwf (@WfRen.wk _ _ _) using 1 <;> autosubst
-    . convert rename_all.2.1 this.2.1 ΔAσwf (@WfRen.wk _ _ _) using 1 <;> autosubst
-    . convert rename_all.2.2.1 this.2.2.1 ΔAσwf (@WfRen.wk _ _ _) using 1 <;> autosubst
+    . convert rename_all.2.1 this.1 ΔAσ (WfRen.wk ..) using 1 <;> autosubst
+    . convert rename_all.2.1 this.2.1 ΔAσ (WfRen.wk ..) using 1 <;> autosubst
+    . convert rename_all.2.2.1 this.2.2.1 ΔAσ (WfRen.wk ..) using 1 <;> autosubst
     . rw [Expr.up_eq_snoc σ, Expr.up_eq_snoc σ']
-      convert rename_all.2.2.2.2 this.2.2.2 ΔAσwf (@WfRen.wk Δ (A.subst σ) l) using 1 <;>
+      convert rename_all.2.2.2.2 this.2.2.2 ΔAσ (WfRen.wk ..) using 1 <;>
         (autosubst; try rw [Expr.comp])
 
 attribute [local grind] WfCtx.snoc wfSb_up_of_eq wfSb_up eqSb_up in
 theorem subst_all :
     (∀ {Γ}, WfCtx Γ → True) ∧
     (∀ {Γ l A}, Γ ⊢[l] A →
-      ∀ {Δ σ}, WfCtx Δ → WfSb Δ σ Γ →
+      ∀ {Δ σ}, WfSb Δ σ Γ →
         (Δ ⊢[l] A.subst σ) ∧
           ∀ {σ'}, WfSb Δ σ' Γ → EqSb Δ σ σ' Γ →
             Δ ⊢[l] A.subst σ ≡ A.subst σ') ∧
     (∀ {Γ l A B}, Γ ⊢[l] A ≡ B →
-      ∀ {Δ σ σ'}, WfCtx Δ → WfSb Δ σ Γ → WfSb Δ σ' Γ → EqSb Δ σ σ' Γ →
+      ∀ {Δ σ σ'}, WfSb Δ σ Γ → WfSb Δ σ' Γ → EqSb Δ σ σ' Γ →
         Δ ⊢[l] A.subst σ ≡ B.subst σ') ∧
     (∀ {Γ l t A}, Γ ⊢[l] t : A →
-      ∀ {Δ σ}, WfCtx Δ → WfSb Δ σ Γ →
+      ∀ {Δ σ}, WfSb Δ σ Γ →
         (Δ ⊢[l] t.subst σ : A.subst σ) ∧
           ∀ {σ'}, WfSb Δ σ' Γ → EqSb Δ σ σ' Γ →
             Δ ⊢[l] t.subst σ ≡ t.subst σ' : A.subst σ) ∧
     (∀ {Γ l t u A}, Γ ⊢[l] t ≡ u : A →
-      ∀ {Δ σ σ'}, WfCtx Δ → WfSb Δ σ Γ → WfSb Δ σ' Γ → EqSb Δ σ σ' Γ →
+      ∀ {Δ σ σ'}, WfSb Δ σ Γ → WfSb Δ σ' Γ → EqSb Δ σ σ' Γ →
         Δ ⊢[l] t.subst σ ≡ u.subst σ' : A.subst σ) := by
   have ih_subst (B a : Expr) (σ) :
       (B.subst a.toSb).subst σ = (B.subst (Expr.up σ)).subst (a.subst σ).toSb := by autosubst
   mutual_induction
   case snoc => exact True.intro
   all_goals try dsimp [Expr.subst] at *
-  case bvar => grind [WfSb, EqSb]
+  case bvar => grind [WfSb.lookup, EqSb.lookup]
   grind_cases
   case pi' => grind [WfTp.pi', EqTp.cong_pi']
   case sigma' => grind [WfTp.sigma', EqTp.cong_sigma']
-  case univ => grind [WfTp.univ, EqTp.refl_tp]
+  case univ => grind [WfSb.wf_dom, WfTp.univ, EqTp.refl_tp]
   case el => grind [WfTp.el, EqTp.cong_el]
   case symm_tp => grind [EqSb.symm, EqTp.symm_tp]
   case trans_tp => grind [EqTp.trans_tp, EqSb.trans, EqSb.refl]
@@ -396,7 +431,9 @@ theorem subst_all :
     . autosubst; grind [wfSb_snoc]
     . autosubst
       rename_i iht _ _ _ _ _ _ _ _
-      apply (iht ..).2 <;> grind [wfSb_snoc, eqSb_snoc]
+
+      sorry
+      -- apply (iht _).2 <;> grind [wfSb_snoc, eqSb_snoc]
     all_goals grind
   case fst_pair' => apply (EqTm.fst_pair' ..).trans_tm' <;> grind
   case snd_pair' =>
@@ -404,14 +441,15 @@ theorem subst_all :
     . autosubst; grind [wfSb_snoc]
     all_goals grind
   case lam_app' ihA ihB ihf _ _ _ Δ σ σ' σσ' =>
-    apply (ihf Δ σ |>.2 σ' σσ').trans_tm' (by grind [WfTp.pi'])
-    have := EqTm.lam_app'
-      (ihA Δ σ').1
-      (ihB (Δ.snoc (by grind))
-      (wfSb_up Δ σ' (by grind))).1
-      (ihf Δ σ').1
-    convert this.conv_tm _ using 3 <;> autosubst
-    grind [EqTp.cong_pi', EqSb.symm, Expr.up_eq_snoc]
+    sorry
+    -- apply (ihf Δ σ |>.2 σ' σσ').trans_tm' (by grind [WfTp.pi'])
+    -- have := EqTm.lam_app'
+    --   (ihA Δ σ').1
+    --   (ihB (Δ.snoc (by grind))
+    --   (wfSb_up Δ σ' (by grind))).1
+    --   (ihf Δ σ').1
+    -- convert this.conv_tm _ using 3 <;> autosubst
+    -- grind [EqTp.cong_pi', EqSb.symm, Expr.up_eq_snoc]
   case pair_fst_snd' =>
     apply (EqTm.pair_fst_snd' ..).trans_tm' <;>
       grind [WfTp.sigma', EqTm.cong_pair', EqTm.cong_fst', EqTm.cong_snd']
